basis/tsFFIScript.sml
@@ -9,23 +9,25 @@ val _ = option_monadsyntax.temp_add_option_monadsyntax();
 
 val _ = Datatype`
   IO_ts = <| latest_time: num;
-             microseconds_elapsed: num -> int
+             microseconds_elapsed: num -> int option
            |>`
 
-Definition getNowMilliseconds_def:
-  getNowMilliseconds ts =
-    let elapsed = ts.microseconds_elapsed 0 in
-    let latest_time = Num (int_max (&(ts.latest_time) + elapsed) 0) in
-    let ts' = <| latest_time := latest_time;
-                 microseconds_elapsed := \n. ts.microseconds_elapsed (n+1) |> in
-    (ts'.latest_time DIV 1000, ts')
+Definition getNow_def:
+  getNow ts =
+    do
+      elapsed <- ts.microseconds_elapsed 0;
+      let latest_time = Num (int_max (&(ts.latest_time) + elapsed) 0) in
+      let ts' = <| latest_time := latest_time;
+                   microseconds_elapsed := ts.microseconds_elapsed o SUC |> in
+      return (ts'.latest_time, ts')
+    od
 End
 
-Definition ffi_get_now_milliseconds_def:
-  ffi_get_now_milliseconds (conf: word8 list) bytes ts =
+Definition ffi_now_def:
+  ffi_now (conf: word8 list) bytes ts =
     do
       assert(9 <= LENGTH bytes);
-      (now, ts') <<- getNowMilliseconds ts;
+      (now, ts') <- getNow ts;
       return (FFIreturn (0w :: n2w8 now ++ (DROP 9 bytes)) ts')
     od ++
     do
@@ -34,70 +36,87 @@ Definition ffi_get_now_milliseconds_def:
     od
 End
 
-Theorem ffi_get_now_milliseconds_length:
-  ffi_get_now_milliseconds conf bytes args = SOME (FFIreturn bytes' args') ⇒
+Theorem ffi_now_length:
+  ffi_now conf bytes args = SOME (FFIreturn bytes' args') ⇒
     LENGTH bytes' = LENGTH bytes
 Proof
-  rw[ffi_get_now_milliseconds_def] \\ fs[option_eq_some]
+  rw[ffi_now_def] \\ fs[option_eq_some]
   \\ TRY(pairarg_tac) \\ rw[] \\ fs[] \\ rw[] \\ fs[n2w8_def]
 QED
 
-Theorem REP_CLASS_11[simp]:
-  int_REP_CLASS i1 = int_REP_CLASS i2 <=> i1 = i2
+(* Theorem REP_CLASS_11[simp]: *)
+(*   int_REP_CLASS i1 = int_REP_CLASS i2 <=> i1 = i2 *)
+(* Proof *)
+(*   metis_tac[integerTheory.int_ABS_REP_CLASS] *)
+(* QED *)
+
+(* Theorem REP_ABS_equiv[simp]: *)
+(*   int_REP_CLASS (int_ABS_CLASS (tint_eq r)) = tint_eq r *)
+(* Proof *)
+(*   simp[GSYM (CONJUNCT2 integerTheory.int_ABS_REP_CLASS)] \\ qexists ‘r’ \\ *)
+(*   fs[integerTheory.TINT_EQ_REFL] *)
+(* QED *)
+
+(* Theorem ABS_CLASS_onto: *)
+(*   !fs. ?r.  fs = int_ABS_CLASS (tint_eq r) *)
+(* Proof *)
+(*   metis_tac[integerTheory.int_ABS_REP_CLASS] *)
+(* QED *)
+
+(* Theorem REP_CLASS_NONEMPTY: *)
+(*   !fs. ?x. int_REP_CLASS fs x *)
+(* Proof *)
+(*   gen_tac >> qspec_then ‘fs’ (qx_choose_then ‘r’ assume_tac) ABS_CLASS_onto >> *)
+(*   simp[] >> metis_tac[integerTheory.TINT_EQ_REFL] *)
+(* QED *)
+
+(* Theorem int_ABS_REP[simp]: *)
+(*   int_ABS (int_REP s) = s *)
+(* Proof *)
+(*   simp[integerTheory.int_REP_def, integerTheory.int_ABS_def] >> *)
+(*   ‘tint_eq ($@ (int_REP_CLASS s)) = int_REP_CLASS s’ *)
+(*     suffices_by metis_tac[REP_CLASS_11, REP_ABS_equiv] >> *)
+(*   simp[FUN_EQ_THM] >> qx_gen_tac ‘a’ >> SELECT_ELIM_TAC >> conj_tac *)
+(*   >- metis_tac[REP_CLASS_NONEMPTY] >> *)
+(*   rw[EQ_IMP_THM] >> *)
+(*   qspec_then ‘s’ (qx_choose_then ‘r’ assume_tac) ABS_CLASS_onto >> fs[] >> *)
+(*   metis_tac[quotientTheory.EQUIV_def, integerTheory.TINT_EQ_EQUIV] *)
+(* QED *)
+
+(* Theorem int_REP_11[simp]: *)
+(*   int_REP i1 = int_REP i2 <=> i1 = i2 *)
+(* Proof *)
+(*   metis_tac[int_ABS_REP] *)
+(* QED *)
+
+Definition Int_def[nocompute]:
+  (Int (n:int)):ffi = Cons (Num (if (n ≥ 0) then 0n else 1n)) (Num (Num n))
+End
+
+Theorem Int_11[simp]:
+  Int x = Int y ⇔ x = y
 Proof
-  metis_tac[integerTheory.int_ABS_REP_CLASS]
+  reverse eq_tac >- fs[Int_def] \\
+  fs[Int_def,integerTheory.Num_EQ] \\
+  rpt IF_CASES_TAC \\ rw[] \\ ‘y = 0’ suffices_by rw[] \\
+  fs[integerTheory.INT_GE_CALCULATE] \\
+  qspecl_then [‘y’,‘0’] mp_tac integerTheory.INT_LE_ANTISYM \\
+  rw[] \\ rw[] \\ rw[] \\
+  fs[integerTheory.INT_NOT_LE] \\ imp_res_tac integerTheory.INT_LT_ANTISYM
 QED
 
-Theorem REP_ABS_equiv[simp]:
-  int_REP_CLASS (int_ABS_CLASS (tint_eq r)) = tint_eq r
-Proof
-  simp[GSYM (CONJUNCT2 integerTheory.int_ABS_REP_CLASS)] \\ qexists ‘r’ \\
-  fs[integerTheory.TINT_EQ_REFL]
-QED
-
-Theorem ABS_CLASS_onto:
-  !fs. ?r.  fs = int_ABS_CLASS (tint_eq r)
-Proof
-  metis_tac[integerTheory.int_ABS_REP_CLASS]
-QED
-
-Theorem REP_CLASS_NONEMPTY:
-  !fs. ?x. int_REP_CLASS fs x
-Proof
-  gen_tac >> qspec_then ‘fs’ (qx_choose_then ‘r’ assume_tac) ABS_CLASS_onto >>
-  simp[] >> metis_tac[integerTheory.TINT_EQ_REFL]
-QED
-
-Theorem int_ABS_REP[simp]:
-  int_ABS (int_REP s) = s
-Proof
-  simp[integerTheory.int_REP_def, integerTheory.int_ABS_def] >>
-  ‘tint_eq ($@ (int_REP_CLASS s)) = int_REP_CLASS s’
-    suffices_by metis_tac[REP_CLASS_11, REP_ABS_equiv] >>
-  simp[FUN_EQ_THM] >> qx_gen_tac ‘a’ >> SELECT_ELIM_TAC >> conj_tac
-  >- metis_tac[REP_CLASS_NONEMPTY] >>
-  rw[EQ_IMP_THM] >>
-  qspec_then ‘s’ (qx_choose_then ‘r’ assume_tac) ABS_CLASS_onto >> fs[] >>
-  metis_tac[quotientTheory.EQUIV_def, integerTheory.TINT_EQ_EQUIV]
-QED
-
-Theorem int_REP_11[simp]:
-  int_REP i1 = int_REP i2 <=> i1 = i2
-Proof
-  metis_tac[int_ABS_REP]
-QED
-
-val dest_iNum_def = Define `
-  dest_iNum (iNum n) = n `;
+Definition dest_iNum_def[nocompute]:
+  dest_iNum (iNum n) = n
+End
 
 (* Packaging up the model as an ffi_part *)
-val encode_def = zDefine‘
-  encode ts = Cons
-              (Num ts.latest_time)
-              (Fun (\ x:ffi_inner.
-                      let elapsed = ts.microseconds_elapsed (dest_iNum x) in
-                      let (elapsed_a, elapsed_b) = int_REP elapsed in
-                      Cons (Num elapsed_a) (Num elapsed_b)))’;
+Definition encode_def[nocompute]:
+  encode ts =
+    Cons
+      (Num ts.latest_time)
+      (Fun (\ x:ffi_inner. Option
+                           (OPTION_MAP Int (ts.microseconds_elapsed (dest_iNum x)))))
+End
 
 Theorem encode_11[simp]:
   !x y. encode x = encode y <=> x = y
@@ -106,11 +125,10 @@ Proof
   fs[FUN_EQ_THM, fetch "-" "IO_ts_component_equality"] \\
   rpt strip_tac \\ last_x_assum (qspec_then ‘iNum x'’ mp_tac) \\
   fs [dest_iNum_def] \\
-  qabbrev_tac ‘f = λ(elapsed_a,elapsed_b). Cons (Num elapsed_a) (Num elapsed_b)’ \\
+  qabbrev_tac ‘f = OPTION_MAP Int’ \\
   qsuff_tac ‘∀a b. f a = f b ⇔ a = b’ >- rw[] \\
-  fs[Abbr‘f’] \\ rpt strip_tac \\ eq_tac
-  >- (Cases_on ‘a’ \\ Cases_on ‘b’ \\ fs[]) \\
-  fs[FUN_EQ_THM]
+  fs[Abbr‘f’] \\ rpt strip_tac \\ reverse eq_tac >- fs[] \\
+  Cases_on ‘a’ \\ Cases_on ‘b’ \\ rw[] \\ rw[] \\ rw[]
 QED
 
 val decode_encode = new_specification("decode_encode",["decode"],
@@ -121,6 +139,6 @@ val _ = export_rewrites ["decode_encode"];
 val ts_ffi_part_def = Define`
   ts_ffi_part =
     (encode,decode,
-      [("get_now_milliseconds",ffi_get_now_milliseconds)])`;
+      [("now",ffi_now)])`;
 
 val _ = export_theory();
