basis/TimeProgScript.sml
@@ -13,55 +13,114 @@ val _ = translation_extends "MarshallingProg";
 
 val _ = ml_prog_update (open_module "Time");
 
+val () = generate_sigs := true;
+
 val _ = ml_prog_update open_local_block;
 
 Datatype:
-  time = Milliseconds num
-End
-
-Definition get_milliseconds_def:
-  get_milliseconds (Milliseconds t) = t
+  time = Time int
 End
 
 val _ = (use_full_type_names := false);
-val _ = register_type ``:time``;
+val _ = register_type “:time”;
 val _ = (use_full_type_names := true);
 
-val _ = (next_ml_names := ["get_milliseconds"]);
-val _ = translate get_milliseconds_def;
-
-val _ = ml_prog_update open_local_block;
-
-val _ = ml_prog_update (add_dec
-  ``Dtabbrev unknown_loc [] "time" (Atapp [] (Short "time"))`` I);
-
-val _ = process_topdecs `
-  exception GetTimeFailed
-` |> append_prog
-
-val _ = ml_prog_update open_local_block;
-
-fun get_exn_conv name =
-  EVAL ``lookup_cons (Short ^name) ^(get_env (get_ml_prog_state ()))``
-  |> concl |> rand |> rand |> rand
-
-val GetTimeFailed = get_exn_conv ``"GetTimeFailed"``;
-
-val GetTimeFailed_exn_def = Define ‘
-  GetTimeFailed_exn v = (v = Conv (SOME ^GetTimeFailed) [])’;
+Definition get_time_def:
+  get_time (Time t) = t
+End
+val _ = (next_ml_names := ["get_time"]);
+val r = translate get_time_def;
 
 val _ = ml_prog_update open_local_in_block;
 
+val _ = ml_prog_update (add_dec
+  “Dtabbrev unknown_loc [] "time" (Atapp [] (Short "time"))” I);
+
+Definition fromMicroseconds_def:
+  fromMicroseconds t = Time t
+End
+
+Definition toMicroseconds_def:
+  toMicroseconds (Time t) = t
+End
+
+val _ = (next_ml_names := ["fromMicroseconds","toMicroseconds"]);
+val r = translate fromMicroseconds_def;
+val r = translate toMicroseconds_def;
+
+Definition fromMilliseconds_def:
+  fromMilliseconds t = Time (t * 1000)
+End
+
+Definition toMilliseconds_def:
+  toMilliseconds (Time t) = t / 1000
+End
+
+val _ = (next_ml_names := ["fromMilliseconds","toMilliseconds"]);
+val r = translate fromMilliseconds_def;
+val r = translate toMilliseconds_def;
+
+Definition fromSeconds_def:
+  fromSeconds t = Time (t * 1000000)
+End
+
+Definition toSeconds_def:
+  toSeconds (Time t) = t / 1000000
+End
+
+val _ = (next_ml_names := ["fromSeconds","toSeconds"]);
+val r = translate fromSeconds_def;
+val r = translate toSeconds_def;
+
+val binopn_lift_def = zDefine ‘
+  binopn_lift (f:int->int->int) =
+    λa b. Time (f (get_time a) (get_time b))’;
+
+fun binopn f_tm =
+  “binopn_lift ^f_tm” |> REWR_CONV binopn_lift_def |> concl |> rhs;
+
+val binopb_lift_def = zDefine ‘
+  binopb_lift (f:int->int->bool) =
+    λa b. f (get_time a) (get_time b)’;
+
+fun binopb f_tm =
+  “binopb_lift ^f_tm” |> REWR_CONV binopb_lift_def |> concl |> rhs;
+
+val _ = trans "+" (binopn intSyntax.plus_tm);
+val _ = trans "-" (binopn intSyntax.minus_tm);
+val _ = trans "*" (binopn intSyntax.mult_tm);
+val _ = trans "div" (binopn intSyntax.div_tm);
+val _ = trans "mod" (binopn intSyntax.mod_tm);
+val _ = trans "<" (binopb intSyntax.less_tm);
+val _ = trans ">" (binopb intSyntax.greater_tm);
+val _ = trans "<=" (binopb intSyntax.leq_tm);
+val _ = trans ">=" (binopb intSyntax.geq_tm);
+val _ = trans "~" “\t. Time (- (get_time t))”;
+
+val _ = process_topdecs ‘exception GetNowFailed’ |> append_prog;
+
+fun get_exn_conv name =
+  EVAL “lookup_cons (Short ^name) ^(get_env (get_ml_prog_state ()))”
+  |> concl |> rand |> rand |> rand
+
+val GetNowFailed = get_exn_conv “"GetNowFailed"”
+
+val _ = ml_prog_update open_local_block;
+
 val _ = process_topdecs ‘
-  fun nowMilliseconds () =
+  fun getNow () =
     let val b = Word8Array.array 9 (Word8.fromInt 0)
-        val a = #(get_now_milliseconds) "" b
+        val a = #(now) "" b
     in
-        if Word8Array.sub b 0 = Word8.fromInt 0
-        then Marshalling.w82n b 1
-        else raise GetTimeFailed
+      if Word8Array.sub b 0 = Word8.fromInt 0
+      then Marshalling.w82n b 1
+      else raise GetNowFailed
     end
 ’ |> append_prog;
+
+val _ = ml_prog_update open_local_in_block
+
+val _ = process_topdecs ‘fun now () = fromMicroseconds (getNow ())’ |> append_prog;
 
 val _ = ml_prog_update close_local_blocks;
 val _ = ml_prog_update (close_module NONE);
